graph.v
@@ -1,0 +1,129 @@
+Require Import Coq.Classes.EquivDec.
+Require Import Coq.Bool.Bool.
+Require Import Lists.ListSet.
+Require Import Coq.Program.Equality.
+
+  
+  Parameter Var : Type.
+  Parameter Lab : Type.
+
+  Parameter Var_dec : EqDec Var eq.
+  Parameter Lab_dec' : forall (l l' : Lab), { l = l' } + { l <> l'}.
+  Parameter Lab_dec : EqDec Lab eq.
+
+  Parameter all_lab : set Lab.
+  Parameter all_lab_spec : forall l, set_In l all_lab.
+
+  Parameter loop_head : Lab -> nat.
+  Parameter loop_exit : Lab -> nat.
+  Parameter is_back_edge : Lab -> Lab -> bool.
+
+  Parameter preds : Lab -> list Lab.
+  Notation "p --> q" := (List.In p (preds q)) (at level 70, right associativity).
+
+  Notation "p -->* q" := (p === q \/ p --> q) (at level 70, right associativity).
+
+  Parameter root : Lab.
+  Parameter root_no_pred : forall p, ~ p --> root.
+
+  Parameter is_def : Var -> Lab -> Lab -> bool.
+
+  Parameter def_edge :
+    forall p q x, is_def x p q = true -> p --> q.
+
+  Definition is_def_lab x p := exists q, is_def x q p = true.
+
+  Lemma Lab_var_dec :
+    forall (x y : (Lab * Var)), { x = y } + { x <> y }.
+  Proof.
+    intros.
+    destruct x as [xa xb], y as [ya yb].
+    destruct ((xa, xb) == (ya, yb)); firstorder.
+  Qed.
+  Program Instance lab_var_eq_eqdec : EqDec (Lab * Var) eq := Lab_var_dec.
+
+  (** Paths **)
+  
+  Inductive Path : Lab -> Lab -> Type :=
+  | PathInit : forall p, Path p p
+  | PathStep : forall from p to, Path from p -> (p --> to) -> Path from to.
+
+  Fixpoint PathIn {a b} (q : Lab) (p : Path a b) : Prop :=
+    match p with
+    | PathInit v => q = v
+    | PathStep from mid to p edge => (q = to) \/ PathIn q p
+    end.
+
+    Lemma Path_in_dec {z a} x (p: Path a z) :
+    {PathIn x p} + {~ PathIn x p}.
+  Proof.
+    induction p.
+    + destruct (x == p); firstorder.
+    + simpl in *. destruct (x == to); firstorder.
+  Qed. 
+
+  Lemma path_first_in {a} b (p : Path a b) :
+    PathIn a p.
+  Proof.
+    induction p.
+    + constructor.
+    + simpl. eauto.
+  Qed.
+
+  Lemma path_last_in {a} b (p : Path a b) :
+    PathIn b p.
+  Proof.
+    induction p.
+    + constructor.
+    + simpl. left. reflexivity.
+  Qed.
+
+  Fixpoint acyclic {a c} (p : Path a c) : Prop :=
+    match p with
+    | PathInit p => True
+    | PathStep a b c p' e => acyclic p' /\ ~ PathIn c p'
+    end.
+
+  Lemma path_in_single_acyclic {a} (p : Path a a) :
+    acyclic p -> forall q, PathIn q p -> q = a.
+  Proof.
+    intros Hacyc q Hin.
+    dependent induction p; simpl in Hin; [ eauto |].
+    simpl in Hacyc.
+    exfalso. apply Hacyc. eapply path_first_in.
+  Qed.
+
+  Lemma acyclic_prefix {a b c} (p : Path a b) (e : b --> c) :
+    acyclic (PathStep a b c p e) -> acyclic p.
+  Proof.
+    intros.
+    destruct p; simpl in *; firstorder.
+  Qed.
+
+  Parameter has_edge_acyclic : Lab -> Lab -> bool.
+  
+  Notation "p '-a>' q" := (has_edge_acyclic p q = true) (at level 70).
+
+  Parameter has_edge_acyclic_spec : forall p q, p -a> q <-> (p --> q
+                                                      /\ (loop_head q = 0
+                                                         \/ loop_exit p = 0)).
+      
+  Lemma has_edge_acyclic_has_edge : forall p q, p -a> q -> p --> q.
+  Proof.
+    intros. apply has_edge_acyclic_spec in H. firstorder.
+  Qed.
+
+  Inductive AcyPath : Lab -> Lab -> Prop :=
+  | AcyPathInit : forall p : Lab, AcyPath p p
+  | AcyPathStep : forall p q r : Lab, AcyPath p q -> q -a> r -> AcyPath p r.
+
+  (*Parameter finite_Lab : 
+    exists (n : nat) (f : Lab -> nat), forall x, f x <= n /\ forall y, f x = f y -> x = y.*) 
+  
+  Parameter dec_path : forall p q, Path p q + (Path p q -> False).
+
+  Definition reaches (p q : Lab) : bool
+    := if dec_path p q then true else false.
+
+
+
